clean up.

dynamic_redblack_btree.v
@@ -861,7 +861,6 @@ Definition balanceR' col l (r : deleted_btree) : deleted_btree :=
     | Black,Bnode Black ll _ (Bleaf _ as lr)
     | Black,Bnode Black ll _ (Bnode Black _ _ _ as lr) =>
       Down (bnode ll (rnode lr r))
-    (* absurd case *)
     | _,_ => Stay (rbnode col l r)
     end
   end.
@@ -869,19 +868,19 @@ Definition balanceR' col l (r : deleted_btree) : deleted_btree :=
 Variable lt_index : nat -> D -> bool.
 Variable right_index : nat -> D -> nat.
 Variable delete_leaf : A -> nat -> A.
-Variable delete_leaves : color -> A -> A -> nat -> deleted_btree.
+Variable delete_from_leaves : color -> A -> A -> nat -> deleted_btree.
 
 Fixpoint bdel B (i : nat) { struct B } : deleted_btree :=
   match B with
-  | Bnode c (Bleaf l) d (Bleaf r) => delete_leaves c l r i
+  | Bnode c (Bleaf l) d (Bleaf r) => delete_from_leaves c l r i
   | Bnode Black (Bnode Red (Bleaf ll) ld (Bleaf lr) as l) d (Bleaf r) =>
     if lt_index i d
     then balanceL' Black (bdel l i) (Bleaf _ r)
     else balanceR' Black (Bleaf _ ll)
-                   (delete_leaves Red lr r (right_index i ld))
+                   (delete_from_leaves Red lr r (right_index i ld))
   | Bnode Black (Bleaf l) ld (Bnode Red (Bleaf rl) rd (Bleaf rr) as r) =>
     if lt_index (right_index i ld) rd
-    then balanceL' Black (delete_leaves Red l rl i) (Bleaf _ rr)
+    then balanceL' Black (delete_from_leaves Red l rl i) (Bleaf _ rr)
     else balanceR' Black (Bleaf _ l) (bdel r (right_index i ld))
   | Bnode c l d r => 
     if lt_index i d
@@ -896,9 +895,9 @@ Definition is_nearly_redblack' tr c bh :=
   | Down tr => is_redblack tr Red bh.-1
   end.
 
-Hypothesis Hdelete_leaves : forall c l d r i c' n,
+Hypothesis Hdelete_from_leaves : forall c l d r i c' n,
   is_redblack (Bnode c (Bleaf D l) d (Bleaf D r)) c' n ->
-  is_nearly_redblack' (delete_leaves c l r i) c' n.
+  is_nearly_redblack' (delete_from_leaves c l r i) c' n.
   
 Lemma is_nearly_redblack'_Red_Black B n :
   is_nearly_redblack' B Red n -> is_nearly_redblack' B Black n.
@@ -942,17 +941,6 @@ Proof.
   repeat decompose_rewrite; by rewrite // !is_redblack_Red_Black. 
 Qed.
   
-Ltac solveL' IHd ok :=
-  rewrite balanceL'_Black_nearly_is_redblack // ?IHd //; decomp ok.
-Ltac solveR' IHd ok :=
-  rewrite balanceR'_Black_nearly_is_redblack // ?IHd //; decomp ok.
-Ltac splitL' t y IHd ok :=
-  case: t => [[] ? ? ?|?] // in y IHd ok *; try by solveL' IHd ok.
-Ltac splitR' t y IHd ok :=
-  case: t => [[] ? ? ?|?] // in y IHd ok *; try by solveR' IHd ok.
-Ltac decomp_ifP ok :=
-  repeat case: ifP => ?; decomp ok.
-
 Ltac close_branch d H IHl IHr :=
  rewrite /=;
  try case:ifP=>?;
@@ -960,17 +948,17 @@ Ltac close_branch d H IHl IHr :=
            balanceR'_Red_nearly_is_redblack,
            balanceL'_Black_nearly_is_redblack,
            balanceR'_Black_nearly_is_redblack,
-           IHl, IHr, Hdelete_leaves (d:=d));
+           IHl, IHr, Hdelete_from_leaves (d:=d));
  decomp H.
 
 Lemma bdel_is_nearly_redblack' B i n c :
   is_redblack B c n -> is_nearly_redblack' (bdel B i) c n.
 Proof.
 elim: B c i n => // c l IHl d r IHr p i n H //.
-time (case: p c l IHl H => [] []// [[]//[[]//???|?]?[[]//???|?]|?] IHl H;
+case: p c l IHl H => [] []// [[]//[[]//???|?]?[[]//???|?]|?] IHl H;
 try (by close_branch d H IHl IHr);
 case: r IHr H => [[]//[[]//???|?]?[[]//???|?]|?] IHr H;
-by close_branch d H IHl IHr).
+by close_branch d H IHl IHr.
 Qed.
 
 End delete.
@@ -992,7 +980,7 @@ Definition deleted_dtree := deleted_btree (nat * nat) (seq bool).
 Local Notation balanceL' c B b := (balanceL' mkD c B b : deleted_dtree).
 Local Notation balanceR' c B b := (balanceR' mkD c B b : deleted_dtree).
 
-Definition delete_leaves (p : color) l r (i : nat) : deleted_dtree :=
+Definition delete_from_leaves (p : color) l r (i : nat) : deleted_dtree :=
   if i < size l
   then match low == size l, low == size r with
        | true,true =>
@@ -1013,25 +1001,25 @@ Definition delete_leaves (p : color) l r (i : nat) : deleted_dtree :=
          Stay (rbnode p (leaf l) (leaf (delete r (i - size l))))
        end.
 
-Lemma delete_leaves_nearly_redblack' c l d r i c' n :
+Lemma delete_from_leaves_nearly_redblack' c l d r i c' n :
   is_redblack (Bnode c (leaf l) d (leaf r)) c' n ->
-  is_nearly_redblack' (delete_leaves c l r i) c' n.
+  is_nearly_redblack' (delete_from_leaves c l r i) c' n.
 Proof.
-  rewrite /delete_leaves.
+  rewrite /delete_from_leaves.
   case: c c' => /= -[]; repeat case: ifP => ?; repeat decompose_rewrite => //=.
 Qed.
 
-Notation ddel := (bdel mkD lt_index right_index (@delete _) delete_leaves).
+Notation ddel := (bdel mkD lt_index right_index (@delete _) delete_from_leaves).
 
 (* Red-blackness invariant *)
 Lemma ddel_is_nearly_redblack' B i n c :
   is_redblack B c n -> is_nearly_redblack' (ddel B i) c n.
-Proof. apply /bdel_is_nearly_redblack' /delete_leaves_nearly_redblack'. Qed.
+Proof. apply /bdel_is_nearly_redblack' /delete_from_leaves_nearly_redblack'. Qed.
 
 (* Correctness lemmas *)
 
 Lemma ddel0E s o l r i :
-  ddel (Bnode Red (leaf l) (s,o) (leaf r)) i = delete_leaves Red l r i.
+  ddel (Bnode Red (leaf l) (s,o) (leaf r)) i = delete_from_leaves Red l r i.
 Proof.
   move Heq : (Bnode Red _ _ _) => B.
   by case: B Heq => [[]//???|?] <-.
@@ -1070,11 +1058,11 @@ Proof.
   by rewrite catA subSn // leqNgt H1.
 Qed.
 
-Lemma delete_leavesE c l r i :
+Lemma delete_from_leavesE c l r i :
   low <= size l < high -> low <= size r < high ->
-  dflattenn (delete_leaves c l r i) = delete (l ++ r) i.
+  dflattenn (delete_from_leaves c l r i) = delete (l ++ r) i.
 Proof.
-  rewrite /delete_leaves delete_cat.
+  rewrite /delete_from_leaves delete_cat.
   case: ifP; case: ifP => //; case: ifP => //;
     try rewrite /delete /= take0 drop1 cat0s cat_rcons -!catA.
       case r => //= /eqP -> /eqP <-; by rewrite ltn0.
@@ -1088,21 +1076,20 @@ Qed.
 Lemma ltn_subLR m n p : 0 < p -> (m - n < p) = (m < n + p).
 Proof. case: p => //= p; by rewrite addnS !ltnS leq_subLR. Qed.
 
-Lemma ddel_cat c l a b r i : 
+Lemma ddel_cat c l a b r i :
   wf_dtree_l (Bnode c l (a, b) r) ->
   dflattenn (ddel (Bnode c l (a, b) r) i) =
   if i < a
   then dflattenn (ddel l i) ++ dflatten r
   else dflatten l ++ dflattenn (ddel r (i - a)).
 Proof.
-  time(
   rewrite /= /lt_index /right_index /=;
   case:ifP=>Hc wfB; case:c l r wfB =>
    [] [[] [??[??]?|?] [??] [??[??]?|?]|?] // [[] [??[??]?|?] [??] [??[??]?|?]|?] wfB;
   try case:ifP;
-  rewrite ?(balanceL'E, balanceR'E, delete_cat, delete_leavesE, ltn_subLR, leq_trans Hlow1);
+  rewrite ?(balanceL'E, balanceR'E, delete_cat, delete_from_leavesE, ltn_subLR, leq_trans Hlow1);
   move:wfB Hc; rewrite ?size_cat;
-  repeat (decompose_rewrite; try by rewrite ltn_addr //) => //=).
+  repeat (decompose_rewrite; try by rewrite ltn_addr //) => //=.
   all: rewrite ?(subnDA, catA) //.
 Qed.
 
@@ -1151,18 +1138,18 @@ Lemma leq_predr (m n : nat) :
   (m == n) = false -> m <= n -> m <= n.-1.
 Proof. rewrite leq_eqVlt => -> /= lo; by rewrite -ltnS (ltn_predK lo). Qed.
 
-Lemma delete_leaves_wf l r i c:
+Lemma delete_from_leaves_wf l r i c:
   i < size l + size r ->
   low <= size l < high ->
   low <= size r < high ->
-  wf_dtree_l (delete_leaves c l r i).
+  wf_dtree_l (delete_from_leaves c l r i).
 Proof.
   move=>sc /andP [wll wlh] /andP [wrl wrh].
   have szl: 0 < size l by apply (leq_trans Hlow1).
   have szr: 0 < size r by apply (leq_trans Hlow1).
   have szlp: (size l).-1 < size l by rewrite prednK // subnn.
   have szrp: (size r).-1 < size r by rewrite prednK // subnn.
-  rewrite /delete_leaves; do! case: ifP; move=>rc lc /=; try (move=> Hi);
+  rewrite /delete_from_leaves; do! case: ifP; move=>rc lc /=; try (move=> Hi);
   rewrite ?(size_cat,size_rcons,size_delete,eqxx) //=;
   rewrite ?(prednK,wll,wlh,wrl,wrh) // -?(eqP rc,eqP lc);
   try (by rewrite leq_addr (leq_trans _ Hlow)// -addnn ltn_add2l prednK);
@@ -1187,32 +1174,32 @@ Proof.
   move => Hn Hi rbB wfB; rewrite dsizeE' // in Hi; move: Hn Hi rbB wfB.
   rewrite /= /lt_index /right_index /=.
   elim:B n i => [[] l IHl [??] r IHr|?] n i Hn Hi rbB wfB /=;
-   last move/eqP:rbB Hn=>/=->//.
+   last by move/eqP:rbB Hn=>/=->.
  +case:ifP => Hc;
   case:l r Hi rbB IHl IHr wfB => [[]?[??]?|?] [[]?[??]?|?] Hi rbB IHl IHr wfB;
   rewrite ?(balanceL'_wf, balanceR'_wf,
-            IHl n, IHr n, delete_leaves_wf, ltn_subLR); 
-  move:rbB wfB Hi Hc; 
+            IHl n, IHr n, delete_from_leaves_wf, ltn_subLR);
+  move:rbB wfB Hi Hc;
   repeat (decompose_rewrite; rewrite /= ?size_cat) => //;
   rewrite ?(ltn_addr, dsize_gt0, leq_trans Hlow1) //=.
-  
+
  +case:n Hn rbB => [//|[//|n]] Hn rbB.
   *case:l r Hi rbB IHl IHr wfB =>
    [[] [[]//=|?] [??] [[]//=|?]|?] [[] [[]//=|?] [??] [[]//=|?]|?] Hi rbB IHl IHr wfB;
-   try case:ifP=>Hc; rewrite ?(balanceL'_wf, balanceR'_wf, delete_leaves_wf) //;
+   try case:ifP=>Hc; rewrite ?(balanceL'_wf, balanceR'_wf, delete_from_leaves_wf) //;
    try move:Hc; move:wfB rbB Hi; repeat (decompose_rewrite; rewrite /= ?size_cat) => //.
    -rewrite ltn_subLR // ltn_addr // (leq_trans Hlow1) //.
    -rewrite ltn_subLR ?addnA // ltn_addr // (leq_trans Hlow1) //.
    -rewrite -ltn_subLR // (leq_trans Hlow1) //.
    -rewrite ltn_subLR // ltn_addr // (leq_trans Hlow1) //.
   *case:l r Hi rbB IHl IHr wfB =>
-   [[] ll [??] lr|?] [[] rl [??] rr|?] Hi rbB IHl IHr wfB;
-   last rewrite delete_leaves_wf //;
+   [[] ll [??] lr|?] [[]?[??]?|?] Hi rbB IHl IHr wfB;
+    last rewrite delete_from_leaves_wf //;
    case:ifP => Hc;
-   try case:ll lr IHl rbB wfB Hi =>[[]???|?] [[]???|?] IHl rbB wfB Hi;
+   try case:ll lr IHl rbB wfB Hi => [[]???|?] [[]???|?] IHl rbB wfB Hi;
    rewrite ?(balanceL'_wf, balanceR'_wf,
-            IHl n.+1, IHr n.+1, delete_leaves_wf, ltn_subLR) //;
-   move:rbB wfB Hi Hc; 
+            IHl n.+1, IHr n.+1, delete_from_leaves_wf, ltn_subLR) //;
+   move:rbB wfB Hi Hc;
    repeat (decompose_rewrite; rewrite /= ?size_cat) => //;
    rewrite ?(ltn_addr, dsize_gt0, leq_trans Hlow1) //=.
 Qed.
@@ -1226,7 +1213,7 @@ Proof.
 case: n => [|n].
   case: B => [[]// [[]//???|s1] [n1 o1] [[]//???|s2]|s] //=.
     move => _ Hi wf.
-    apply /wf_dtree_dtree' /delete_leaves_wf => //; by decomp wf.
+    apply /wf_dtree_dtree' /delete_from_leaves_wf => //; by decomp wf.
   move=> _ Hi Hs; rewrite size_delete //.
   by rewrite (ltn_predK Hi) ltnW.
 case: B => // c l d r rb Hi wf.
